proofs/talos/lean/Project/Beck/AnnotationMatches.lean
@@ -23,80 +23,104 @@ set_option maxHeartbeats 8000000
 
 namespace Project.Beck.AnnotationMatches
 
-def function_18_erase_copy_0_prefix_program : Wasm.Program :=
+def function_2_while_loop_0_guard_program : Wasm.Program :=
+  Project.ProofKit.FuelGuard.program 0 12
+
+theorem function_2_while_loop_0_guard_eq :
+    Project.ProofKit.Annotation.region Project.Beck.func2
+      [{ instructionIndex := 6, field := .block }, { instructionIndex := 0, field := .loop }] 0 7 = some function_2_while_loop_0_guard_program := by
+  rfl
+
+theorem function_2_while_loop_0_guard_tail_eq :
+    (Project.ProofKit.Annotation.resolve Project.Beck.func2 [{ instructionIndex := 6, field := .block }, { instructionIndex := 0, field := .loop }]).getD [] = function_2_while_loop_0_guard_program ++ ((Project.ProofKit.Annotation.resolve Project.Beck.func2 [{ instructionIndex := 6, field := .block }, { instructionIndex := 0, field := .loop }]).getD []).drop 7 := by
+  rfl
+
+def function_5_while_loop_0_guard_program : Wasm.Program :=
+  Project.ProofKit.FuelGuard.program 0 15
+
+theorem function_5_while_loop_0_guard_eq :
+    Project.ProofKit.Annotation.region Project.Beck.func5
+      [{ instructionIndex := 6, field := .block }, { instructionIndex := 0, field := .loop }] 0 7 = some function_5_while_loop_0_guard_program := by
+  rfl
+
+theorem function_5_while_loop_0_guard_tail_eq :
+    (Project.ProofKit.Annotation.resolve Project.Beck.func5 [{ instructionIndex := 6, field := .block }, { instructionIndex := 0, field := .loop }]).getD [] = function_5_while_loop_0_guard_program ++ ((Project.ProofKit.Annotation.resolve Project.Beck.func5 [{ instructionIndex := 6, field := .block }, { instructionIndex := 0, field := .loop }]).getD []).drop 7 := by
+  rfl
+
+def function_23_erase_copy_0_prefix_program : Wasm.Program :=
   Project.ProofKit.FixedArrayCopy.prefixProgram
     8 14
     11 15
 
-def function_18_erase_copy_0_suffix_program : Wasm.Program :=
+def function_23_erase_copy_0_suffix_program : Wasm.Program :=
   Project.ProofKit.FixedArrayCopy.suffixProgram
     1 8 14
     11 12
     15
 
-def function_18_erase_copy_0_program : Wasm.Program :=
+def function_23_erase_copy_0_program : Wasm.Program :=
   Project.ProofKit.FixedArrayCopy.program
     1 8 14
     11 12
     15
 
-theorem function_18_erase_copy_0_prefix_eq :
-    Project.ProofKit.Annotation.region Project.Beck.func18
+theorem function_23_erase_copy_0_prefix_eq :
+    Project.ProofKit.Annotation.region Project.Beck.func23
       [{ instructionIndex := 15, field := .thenBranch }] 53
-      56 = some function_18_erase_copy_0_prefix_program := by
+      56 = some function_23_erase_copy_0_prefix_program := by
   rfl
 
-theorem function_18_erase_copy_0_suffix_eq :
-    Project.ProofKit.Annotation.region Project.Beck.func18
+theorem function_23_erase_copy_0_suffix_eq :
+    Project.ProofKit.Annotation.region Project.Beck.func23
       [{ instructionIndex := 15, field := .thenBranch }] 56
-      59 = some function_18_erase_copy_0_suffix_program := by
+      59 = some function_23_erase_copy_0_suffix_program := by
   rfl
 
-theorem function_18_erase_copy_0_eq :
-    Project.ProofKit.Annotation.region Project.Beck.func18
+theorem function_23_erase_copy_0_eq :
+    Project.ProofKit.Annotation.region Project.Beck.func23
       [{ instructionIndex := 15, field := .thenBranch }] 53
-      59 = some function_18_erase_copy_0_program := by
+      59 = some function_23_erase_copy_0_program := by
   rfl
 
-theorem function_18_erase_copy_0_tail_eq :
-    ((Project.ProofKit.Annotation.resolve Project.Beck.func18 [{ instructionIndex := 15, field := .thenBranch }]).getD []).drop 53 =
-      Project.Beck.AnnotationMatches.function_18_erase_copy_0_program ++ ((Project.ProofKit.Annotation.resolve Project.Beck.func18 [{ instructionIndex := 15, field := .thenBranch }]).getD []).drop 59 := by
+theorem function_23_erase_copy_0_tail_eq :
+    ((Project.ProofKit.Annotation.resolve Project.Beck.func23 [{ instructionIndex := 15, field := .thenBranch }]).getD []).drop 53 =
+      Project.Beck.AnnotationMatches.function_23_erase_copy_0_program ++ ((Project.ProofKit.Annotation.resolve Project.Beck.func23 [{ instructionIndex := 15, field := .thenBranch }]).getD []).drop 59 := by
   rfl
 
-def function_19_while_loop_0_guard_program : Wasm.Program :=
+def function_24_while_loop_0_guard_program : Wasm.Program :=
   Project.ProofKit.FuelGuard.program 0 12
 
-theorem function_19_while_loop_0_guard_eq :
-    Project.ProofKit.Annotation.region Project.Beck.func19
-      [{ instructionIndex := 8, field := .block }, { instructionIndex := 0, field := .loop }] 0 7 = some function_19_while_loop_0_guard_program := by
+theorem function_24_while_loop_0_guard_eq :
+    Project.ProofKit.Annotation.region Project.Beck.func24
+      [{ instructionIndex := 8, field := .block }, { instructionIndex := 0, field := .loop }] 0 7 = some function_24_while_loop_0_guard_program := by
   rfl
 
-theorem function_19_while_loop_0_guard_tail_eq :
-    (Project.ProofKit.Annotation.resolve Project.Beck.func19 [{ instructionIndex := 8, field := .block }, { instructionIndex := 0, field := .loop }]).getD [] = function_19_while_loop_0_guard_program ++ ((Project.ProofKit.Annotation.resolve Project.Beck.func19 [{ instructionIndex := 8, field := .block }, { instructionIndex := 0, field := .loop }]).getD []).drop 7 := by
+theorem function_24_while_loop_0_guard_tail_eq :
+    (Project.ProofKit.Annotation.resolve Project.Beck.func24 [{ instructionIndex := 8, field := .block }, { instructionIndex := 0, field := .loop }]).getD [] = function_24_while_loop_0_guard_program ++ ((Project.ProofKit.Annotation.resolve Project.Beck.func24 [{ instructionIndex := 8, field := .block }, { instructionIndex := 0, field := .loop }]).getD []).drop 7 := by
   rfl
 
-def function_22_while_loop_0_guard_program : Wasm.Program :=
+def function_27_while_loop_0_guard_program : Wasm.Program :=
   Project.ProofKit.FuelGuard.program 0 17
 
-theorem function_22_while_loop_0_guard_eq :
-    Project.ProofKit.Annotation.region Project.Beck.func22
-      [{ instructionIndex := 8, field := .block }, { instructionIndex := 0, field := .loop }] 0 7 = some function_22_while_loop_0_guard_program := by
+theorem function_27_while_loop_0_guard_eq :
+    Project.ProofKit.Annotation.region Project.Beck.func27
+      [{ instructionIndex := 8, field := .block }, { instructionIndex := 0, field := .loop }] 0 7 = some function_27_while_loop_0_guard_program := by
   rfl
 
-theorem function_22_while_loop_0_guard_tail_eq :
-    (Project.ProofKit.Annotation.resolve Project.Beck.func22 [{ instructionIndex := 8, field := .block }, { instructionIndex := 0, field := .loop }]).getD [] = function_22_while_loop_0_guard_program ++ ((Project.ProofKit.Annotation.resolve Project.Beck.func22 [{ instructionIndex := 8, field := .block }, { instructionIndex := 0, field := .loop }]).getD []).drop 7 := by
+theorem function_27_while_loop_0_guard_tail_eq :
+    (Project.ProofKit.Annotation.resolve Project.Beck.func27 [{ instructionIndex := 8, field := .block }, { instructionIndex := 0, field := .loop }]).getD [] = function_27_while_loop_0_guard_program ++ ((Project.ProofKit.Annotation.resolve Project.Beck.func27 [{ instructionIndex := 8, field := .block }, { instructionIndex := 0, field := .loop }]).getD []).drop 7 := by
   rfl
 
-def function_29_while_loop_0_guard_program : Wasm.Program :=
+def function_34_while_loop_0_guard_program : Wasm.Program :=
   Project.ProofKit.FuelGuard.program 0 15
 
-theorem function_29_while_loop_0_guard_eq :
-    Project.ProofKit.Annotation.region Project.Beck.func29
-      [{ instructionIndex := 6, field := .block }, { instructionIndex := 0, field := .loop }] 0 7 = some function_29_while_loop_0_guard_program := by
+theorem function_34_while_loop_0_guard_eq :
+    Project.ProofKit.Annotation.region Project.Beck.func34
+      [{ instructionIndex := 6, field := .block }, { instructionIndex := 0, field := .loop }] 0 7 = some function_34_while_loop_0_guard_program := by
   rfl
 
-theorem function_29_while_loop_0_guard_tail_eq :
-    (Project.ProofKit.Annotation.resolve Project.Beck.func29 [{ instructionIndex := 6, field := .block }, { instructionIndex := 0, field := .loop }]).getD [] = function_29_while_loop_0_guard_program ++ ((Project.ProofKit.Annotation.resolve Project.Beck.func29 [{ instructionIndex := 6, field := .block }, { instructionIndex := 0, field := .loop }]).getD []).drop 7 := by
+theorem function_34_while_loop_0_guard_tail_eq :
+    (Project.ProofKit.Annotation.resolve Project.Beck.func34 [{ instructionIndex := 6, field := .block }, { instructionIndex := 0, field := .loop }]).getD [] = function_34_while_loop_0_guard_program ++ ((Project.ProofKit.Annotation.resolve Project.Beck.func34 [{ instructionIndex := 6, field := .block }, { instructionIndex := 0, field := .loop }]).getD []).drop 7 := by
   rfl
 
 end Project.Beck.AnnotationMatches
